refactor

Logic/Logic/HilbertStyle2.lean
@@ -19,7 +19,7 @@ variable (Bew : Finset F → F → Sort*)
   Minimal Propositional Logic.
 -/
 class Minimal [NegDefinition F] extends Deduction Bew where
-  modus_ponens {Γ : Finset F} {p q : F}   : (Bew Γ (p ⟶ q)) → (Bew Γ p) → (Bew Γ q)
+  modus_ponens {Γ₁ Γ₂ : Finset F} {p q : F} : (Bew Γ₁ (p ⟶ q)) → (Bew Γ₂ p) → (Bew (Γ₁ ∪ Γ₂) q)
   verum        (Γ : Finset F)             : Bew Γ ⊤
   imply₁       (Γ : Finset F) (p q : F)   : Bew Γ (p ⟶ (q ⟶ p))
   imply₂       (Γ : Finset F) (p q r : F) : Bew Γ ((p ⟶ q ⟶ r) ⟶ (p ⟶ q) ⟶ p ⟶ r)
@@ -32,7 +32,7 @@ class Minimal [NegDefinition F] extends Deduction Bew where
 
 /-- Supplymental -/
 class HasDT where
-  dt {Γ : Finset F} {p q : F} : (Bew (insert p Γ) q) → (Bew Γ (p ⟶ q))
+  dtr {Γ : Finset F} {p q : F} : (Bew (insert p Γ) q) → (Bew Γ (p ⟶ q))
 
 class HasEFQ where
   efq (Γ : Finset F) (p : F) : Bew Γ (⊥ ⟶ p)
@@ -83,9 +83,9 @@ class Classical extends Minimal Bew, HasDNE Bew
 
 end
 
-open Deduction Minimal HasDT Intuitionistic Classical
+open Deduction Minimal HasDT Intuitionistic Classical HasDNE
 
-infixl:90 " ⨀ " => modus_ponens
+infixr:90 " ⨀ " => modus_ponens
 
 variable {Bew : Finset F → F → Sort*} (Γ : Finset F) (p q r : F)
 
@@ -93,29 +93,19 @@ section Minimal
 
 variable [hM : Minimal Bew] [HasDT Bew]
 
-/-
-lemma imply₁ : Bew Γ (p ⟶ (q ⟶ p)) := by
-  repeat apply dtr;
-  apply axm;
-  simp;
+def modus_ponens' {Γ p q} (d₁ : Bew Γ (p ⟶ q)) (d₂ : Bew Γ p) : Bew Γ q := by simpa using d₁ ⨀ d₂
 
-lemma imply₂ : Bew Γ ((p ⟶ q ⟶ r) ⟶ (p ⟶ q) ⟶ p ⟶ r) := by
-  repeat apply dtr;
-  have h₁ : Bew (insert p (insert (p ⟶ q) (insert (p ⟶ q ⟶ r) Γ))) p := axm (by simp);
-  have h₂ : Bew (insert p (insert (p ⟶ q) (insert (p ⟶ q ⟶ r) Γ))) (p ⟶ q) := axm (by simp);
-  have h₃ : Bew (insert p (insert (p ⟶ q) (insert (p ⟶ q ⟶ r) Γ))) (p ⟶ q ⟶ r) := axm (by simp);
-  exact (h₃ ⨀ h₁) ⨀ (h₂ ⨀ h₁);
--/
+infixr:90 " ⨀ " => modus_ponens'
 
-lemma dtl (d : Bew Γ (p ⟶ q)) : Bew (insert p Γ) q := (weakening' (by simp) d) ⨀ (axm (by simp))
+def dtl {Γ p q} (d : Bew Γ (p ⟶ q)) : Bew (insert p Γ) q := (weakening' (by simp) d) ⨀ (axm (by simp))
 
 @[simp]
-lemma imp_id : Bew Γ (p ⟶ p) := (imply₂ Γ p (p ⟶ p) p) ⨀ (imply₁ _ _ _) ⨀ (imply₁ _ _ _)
+lemma imp_id : Bew Γ (p ⟶ p) := ((imply₂ Γ p (p ⟶ p) p) ⨀ (imply₁ _ _ _)) ⨀ (imply₁ _ _ _)
 
 lemma dni : Bew Γ (p ⟶ ~~p) := by
   have h₁ : Bew (insert (p ⟶ ⊥) (insert p Γ)) (p ⟶ ⊥) := axm (by simp);
   have h₂ : Bew (insert (p ⟶ ⊥) (insert p Γ)) p := axm (by simp);
-  simpa using dt $ dt $ h₁ ⨀ h₂;
+  simpa using dtr $ dtr $ h₁ ⨀ h₂;
 
 end Minimal
 
@@ -126,12 +116,9 @@ variable [c : Classical Bew] [HasDT Bew]
 
 instance : HasEFQ Bew where
   efq Γ p := by
-    have h₁ : Bew (insert ⊥ Γ) ⊥ := axm (by simp);
-    have h₂ := c.imply₁ (insert ⊥ Γ) ⊥ (p ⟶ ⊥);
-    have h₃ := h₂ ⨀ h₁;
-    have h₄ := c.dne (insert ⊥ Γ) p;
-    have h₅ := (by simpa using h₄) ⨀ h₃;
-    exact dt h₅;
+    have h₁ : Bew (insert ⊥ Γ) (⊥ ⟶ (p ⟶ ⊥) ⟶ ⊥) := imply₁ (insert ⊥ Γ) ⊥ (p ⟶ ⊥);
+    have h₂ : Bew (insert ⊥ Γ) (((p ⟶ ⊥) ⟶ ⊥) ⟶ p) := by simpa using dne (insert ⊥ Γ) p;
+    exact dtr $ h₂ ⨀ h₁ ⨀ (axm (by simp));
 
 instance : Intuitionistic Bew where
 
