Logic/Modal/Normal/Soundness.lean
@@ -2,39 +2,45 @@ import Logic.Modal.Normal.Formula
 import Logic.Modal.Normal.HilbertStyle
 import Logic.Modal.Normal.Semantics
 
+attribute [simp] Finset.union_eq_empty
+
 namespace LO.Modal.Normal
 
 open Formula
 
+variable {α β} [Inhabited α] [DecidableEq α] [Inhabited β]
+
 @[simp]
-def AxiomSet.Consistent {α} (Λ : AxiomSet α) := ⊬ᴹ[Λ]! ⊥
+def AxiomSet.Consistent (Λ : AxiomSet α) := ⊬ᴹ[Λ]! ⊥
 
 open AxiomSet
 
-variable {α β} [Inhabited α] [Inhabited β] {Λ : AxiomSet α} {p : Formula α}
+variable  {Λ : AxiomSet α} {Γ : Context α} {p : Formula α}
 
-lemma AxiomSet.sounds (h : ⊢ᴹ[Λ] p) : (⊧ᴹ[(𝔽(Λ) : FrameClass β)] p) := by
-  induction h <;> try { simp [FrameClasses, Frames, Models]; try intros; aesop; }
-  case modus_ponens ih₁ ih₂ => exact FrameClasses.modus_ponens ih₁ ih₂;
+private lemma AxiomSet.sounds' (Γ) (_ : Γ = ∅) (h : Deducible Λ Γ p) : (⊧ᴹ[(𝔽(Λ) : FrameClass β)] p) := by
+  induction h.some <;> try { simp [FrameClasses, Frames, Models]; try intros; aesop; }
+  case modus_ponens h₁ h₂ ih₁ ih₂ he => exact FrameClasses.modus_ponens (ih₁ (by aesop) ⟨h₁⟩) (ih₂ (by aesop) ⟨h₂⟩);
+
+lemma AxiomSet.sounds (h : ⊢ᴹ[Λ]! p) : (⊧ᴹ[(𝔽(Λ) : FrameClass β)] p) := AxiomSet.sounds' ∅ rfl h
 
 lemma AxiomSet.consistent (β) [Inhabited β] [h : Nonempty (𝔽(Λ) : FrameClass β)] : Consistent Λ := by
   by_contra hC; simp at hC;
   suffices h : ∃ (F : Frame β), ⊧ᴹ[F] (⊥ : Formula α) by aesop;
   have ⟨tf, htf⟩ := h.some;
   existsi tf;
-  apply AxiomSet.sounds hC.some;
+  apply AxiomSet.sounds hC;
   assumption;
 
-theorem LogicK.sounds : (⊢ᴹ[𝐊] p) → (⊧ᴹ[(𝔽((𝐊 : AxiomSet α)) : FrameClass β)] p) := by apply AxiomSet.sounds;
+theorem LogicK.sounds : (⊢ᴹ[𝐊]! p) → (⊧ᴹ[(𝔽((𝐊 : AxiomSet α)) : FrameClass β)] p) := by apply AxiomSet.sounds;
 theorem LogicK.consistent : Consistent (𝐊 : AxiomSet α) := AxiomSet.consistent β
 
-theorem LogicKD.sounds : (⊢ᴹ[𝐊𝐃] p) → (⊧ᴹ[(𝔽((𝐊𝐃 : AxiomSet α)) : FrameClass β)] p) := by apply AxiomSet.sounds;
+theorem LogicKD.sounds : (⊢ᴹ[𝐊𝐃]! p) → (⊧ᴹ[(𝔽((𝐊𝐃 : AxiomSet α)) : FrameClass β)] p) := by apply AxiomSet.sounds;
 theorem LogicKD.consistent : Consistent (𝐊𝐃 : AxiomSet α) := AxiomSet.consistent β
 
-theorem LogicS4.sounds : (⊢ᴹ[𝐒𝟒] p) → (⊧ᴹ[(𝔽((𝐒𝟒 : AxiomSet α)) : FrameClass β)] p) := by apply AxiomSet.sounds;
+theorem LogicS4.sounds : (⊢ᴹ[𝐒𝟒]! p) → (⊧ᴹ[(𝔽((𝐒𝟒 : AxiomSet α)) : FrameClass β)] p) := by apply AxiomSet.sounds;
 theorem LogicS4.consistent : Consistent (𝐒𝟒 : AxiomSet α) := AxiomSet.consistent β
 
-theorem LogicS5.sounds : (⊢ᴹ[𝐒𝟓] p) → (⊧ᴹ[(𝔽((𝐒𝟓 : AxiomSet α)) : FrameClass β)] p) := by apply AxiomSet.sounds;
+theorem LogicS5.sounds : (⊢ᴹ[𝐒𝟓]! p) → (⊧ᴹ[(𝔽((𝐒𝟓 : AxiomSet α)) : FrameClass β)] p) := by apply AxiomSet.sounds;
 theorem LogicS5.consistent : Consistent (𝐒𝟓 : AxiomSet α) := AxiomSet.consistent β
 
 /-
